Basic setup for non-dependent hash map

Hashmap/HashMap/Basic.lean
@@ -1,1 +1,61 @@
-import HashMap.DHashMap.Basic
+/-
+Copyright (c) 2024 Lean FRO, LLC. All rights reserved.
+Released under Apache 2.0 license as described in the file LICENSE.
+Authors: Markus Himmel
+-/
+import Hashmap.DHashMap.Basic
+import Hashmap.Sigma
+
+set_option autoImplicit false
+
+universe u v
+
+variable {α : Type u} {β : Type v}
+
+namespace MyLean
+
+namespace HashMap
+
+structure Raw (α : Type u) (β : Type v) where
+  raw : DHashMap.Raw α (fun _ => β)
+
+namespace Raw
+
+@[inline] def empty (capacity := 8) : Raw α β :=
+  ⟨DHashMap.Raw.empty capacity⟩
+
+@[inline] def insert' [BEq α] [Hashable α] (m : Raw α β) (a : α) (b : β) : Raw α β × Bool :=
+  let ⟨r, replaced⟩ := m.raw.insert' a b
+  ⟨⟨r⟩, replaced⟩
+
+@[inline] def insert [BEq α] [Hashable α] (m : Raw α β) (a : α) (b : β) : Raw α β :=
+  ⟨m.raw.insert a b⟩
+
+@[inline] def findEntry? [BEq α] [Hashable α] (m : Raw α β) (a : α) : Option (α × β) :=
+  m.raw.findEntry? a |> .map Sigma.toProd
+
+def WF [BEq α] [Hashable α] : Raw α β → Prop :=
+  fun r => r.raw.WF
+
+end Raw
+
+end HashMap
+
+def HashMap (α : Type u) (β : Type v) [BEq α] [Hashable α] :=
+  DHashMap α (fun _ => β)
+
+namespace HashMap
+
+@[inline] def empty [BEq α] [Hashable α] (capacity := 8) : HashMap α β :=
+  DHashMap.empty capacity
+
+@[inline] def insert' [BEq α] [Hashable α] (m : HashMap α β) (a : α) (b : β) : HashMap α β × Bool :=
+  DHashMap.insert' m a b
+
+@[inline] def insert [BEq α] [Hashable α] (m : HashMap α β) (a : α) (b : β) : HashMap α β :=
+  DHashMap.insert m a b
+
+@[inline] def findEntry? [BEq α] [Hashable α] (m : HashMap α β) (a : α) : Option (α × β) :=
+  DHashMap.findEntry? m a |> .map Sigma.toProd
+
+end MyLean.HashMap
