Hashmap/HashMap/Lemmas.lean
@@ -1,0 +1,33 @@
+/-
+Copyright (c) 2024 Lean FRO, LLC. All rights reserved.
+Released under Apache 2.0 license as described in the file LICENSE.
+Authors: Markus Himmel
+-/
+import Hashmap.DHashMap.Lemmas
+import Hashmap.HashMap.Basic
+
+set_option autoImplicit false
+
+universe u v
+
+variable {α : Type u} {β : Type v}
+
+namespace MyLean.HashMap
+
+namespace Raw
+
+theorem ext (m m' : Raw α β) : m.raw = m'.raw → m = m' := by
+  cases m; cases m'; rintro rfl; rfl
+
+theorem findEntry?_insert [BEq α] [Hashable α] [EquivBEq α] [LawfulHashable α] (m : Raw α β) (h : m.WF) {a k : α} {b : β} :
+    (m.insert a b).findEntry? k = bif a == k then some (a, b) else m.findEntry? k := by
+  rw [findEntry?, insert, findEntry?, DHashMap.Raw.findEntry?_insert _ h]
+  simp [apply_bif (Option.map Sigma.toProd)]
+
+end Raw
+
+theorem findEntry?_insert [BEq α] [Hashable α] [EquivBEq α] [LawfulHashable α] (m : HashMap α β) {a k : α} {b : β} :
+    (m.insert a b).findEntry? k = bif a == k then some (a, b) else m.findEntry? k := by
+  simp [findEntry?, insert, DHashMap.findEntry?_insert, apply_bif (Option.map Sigma.toProd)]
+
+end MyLean.HashMap
